proof of correctness of strlen, main lemma

c/poc/sandbox.v
@@ -137,3 +137,375 @@ Lemma strlen_correct_with_C_string : Archi.ptr64 = false -> forall ge e m b ofs 
                (le'!_output) = Some (VintN len).
 (* the C light expression evaluates to outcome Out_return (Some VintN len) and output is set to len *)
 Admitted.
+
+
+(* non-empty string *)
+Lemma strlen_loop_continue_correct : Archi.ptr64 = false -> forall len ge e m b ofs le,
+      
+      1 <= Z.of_nat (S len) < Ptrofs.modulus ->
+      ofs + Z.of_nat (S len) < Ptrofs.modulus ->
+      0 < ofs < Ptrofs.modulus ->
+      0 <= Z.of_nat (S len) < Ptrofs.modulus ->
+
+      strlen_mem m b ofs (S len) -> (* assume we have a string of length (S len) at [b,ofs] in m *)
+      
+      forall i, (i < S len)%nat ->  (* then the loop continues until len and outputs i++ *)
+           
+      le!_input = Some (Vptr b (Ptrofs.repr (ofs + Z.of_nat i))) -> 
+      le!_output = Some (VintN i) ->
+      
+      exists t, exec_stmt ge e le m f_strlen_loop t (Maps.PTree.set _output (VintN (S i)) le) m Out_normal.
+Proof.
+  induction len.
+  -  (* Base case *)
+    intros. assert (i = 0)%nat by omega. rewrite H8 in *. replace (ofs + Z.of_nat 0) with ofs in H6 by nia. inversion_clear H4.
+   destruct (strlen_loop_break_correct2 H ge e m b ofs 1 (PTree.set _output (VintN 1) le)). 
+        1-3: nia.
+        repeat gso_assumption.
+        apply gss.
+        simpl.
+        inversion H9.
+        assumption.   
+        eexists.
+        loop. repeat econstructor. repeat gso_assumption. gso_assumption.   repeat econstructor. simpl. replace (Ptrofs.unsigned (Ptrofs.add (Ptrofs.repr ofs) (Ptrofs.mul (Ptrofs.repr 1) (Ptrofs.of_intu (Int.repr 0))))) with ofs. apply H10.  { pose (Ptrofs.modulus_eq32 H). ptrofs_compute_add_mul. all: nia. } repeat econstructor. simpl. repeat econstructor. simpl.
+        replace (negb (Int.eq (Int.repr (Z.pos v)) (Int.repr 0))) with true.      
+        econstructor. admit. repeat econstructor. repeat econstructor. repeat econstructor.
+        gso_assumption. repeat econstructor.
+        fold f_strlen_loop.
+        replace (Int.add (Int.repr (Z.of_nat 0)) (Int.repr 1)) with (Int.repr 1) by (auto with ints).      apply H4.
+    
+  - induction i ; intros. replace (ofs + Z.of_nat 0) with ofs in * by nia.
+    inversion_clear H4. 
+    eexists.
+    
+        loop. repeat econstructor. repeat gso_assumption. gso_assumption. repeat econstructor. simpl. replace (Ptrofs.unsigned (Ptrofs.add (Ptrofs.repr ofs) (Ptrofs.mul (Ptrofs.repr 1) (Ptrofs.of_intu (Int.repr 0))))) with ofs. apply H9.  { pose (Ptrofs.modulus_eq32 H). ptrofs_compute_add_mul. all: nia. } repeat econstructor. simpl. repeat econstructor. simpl.
+        replace (negb (Int.eq (Int.repr (Z.pos v)) (Int.repr 0))) with true.      
+        econstructor. admit. repeat econstructor. repeat econstructor. repeat econstructor.
+        gso_assumption. repeat econstructor.
+        
+        fold f_strlen_loop.
+        
+        replace (Int.add (Int.repr (Z.of_nat 0)) (Int.repr 1)) with (Int.repr 1) by (auto with ints).
+         replace ofs with  (ofs + Z.of_nat 0) in H6 by nia.
+         assert (exists t : trace,
+   exec_stmt ge e le m f_strlen_loop t (PTree.set _output (VintN 1) le) m Out_normal).
+
+    (*     refine  (IHlen ge e m b ofs le _ _ _ _ _ O _ H6 H7).
+         1-4: nia.
+         
+        destruct (strlen_loop_break_correct2 H ge e m b ofs 1 (PTree.set _output (VintN 1) le)). 
+        1-3: nia.
+        repeat gso_assumption.
+        apply gss.
+        simpl.
+        inversion_clear H8.
+        (* wrong : Mem.load Mint8signed m b (ofs + 1) = Some (VintP v0) with v0 positive *)
+        assumption.  
+
+        apply H4.
+    
+    + intros. inversion_clear H4.
+      pose (IHlen ge e m b (ofs + 1) le).
+      assert (1 <= Z.of_nat (S len) < Ptrofs.modulus) by nia. 
+      assert (ofs + 1 + Z.of_nat (S len) < Ptrofs.modulus) by nia.
+      assert (0 < ofs + 1 < Ptrofs.modulus) by nia.
+      assert (0 <= Z.of_nat (S len) < Ptrofs.modulus) by nia.
+      apply (e0 H4 H10 H11 H12).
+      assumption.
+      admit. (* (0 < len)%nat *) 
+      admit. (* le ! _input = Some (Vptr b (Ptrofs.repr (ofs + 1))) *)
+      assumption.
+    +   *)
+       
+Admitted.
+
+
+Lemma exec_trans : forall ge e le m t b ofs outp,
+    le!_output = Some (VintZ 0) ->
+    exec_stmt ge e (PTree.set _input (Vptr b (Ptrofs.repr (ofs + 1))) le) m f_strlen_loop t  (PTree.set _output (VintN outp)(PTree.set _input (Vptr b (Ptrofs.repr (ofs + 1))) le)) m Out_normal ->
+
+    le ! _input = Some (Vptr b (Ptrofs.repr ofs)) ->
+    exec_stmt ge e (PTree.set _output (VintZ 1) le) m f_strlen_loop t (PTree.set _output (VintN outp) le) m Out_normal. 
+  Admitted.
+
+
+                        
+(* Old stuff: One direction of correctness, using functional spec, below relational with proof attempt *)
+
+ Definition strlen_C_fun_corr_r :
+  forall (ge :genv) (m : Mem.mem) (b : block) (ofs : Z) (e : env) (le : temp_env) (z : Z),
+    strlen_C_fun_spec m b ofs = Some (z,m) ->
+    le!_s = Some (Vptr b (Ptrofs.repr ofs)) -> (* input parameter _s assigned value of address (b,ofs) in le *)
+    exists t le', exec_stmt ge e le m f_strlen.(fn_body) t le' m (Out_return (Some (Vint (Int.repr z),tuint))) /\ le'!_i = Some (Vint (Int.repr z)).
+               (* in environments ge, e (local env), le and memory m with output trace t, output _i assigned value z *)
+Admitted.
+
+ (* Find proofs on arithmetic on ptrofs type to rewrite this *)
+      Hypothesis ptr_ofs_eq : forall ofs, ofs = (Ptrofs.unsigned
+       (Ptrofs.add (Ptrofs.repr ofs)
+                   (Ptrofs.mul (Ptrofs.repr 1) (Ptrofs.of_intu (Int.repr 0))))). 
+
+      
+Definition strlen_C_rel_corr_r : forall n m b ofs e le ge,
+    strlen_C_rel_spec m b ofs (Some (n,m)) ->
+    le!_s = Some (Vptr b (Ptrofs.repr ofs)) -> 
+    exists t le', le'!_i = Some (Vint_of_nat n) /\ 
+           exec_stmt ge e le m f_strlen.(fn_body) t le' m (Out_return (Some ((Vint_of_nat n),tuint))).
+Proof.
+  induction n.
+  (* Base case. *)
+    intros.
+    inversion H. unfold chunk in *. destruct H4.
+    eexists.
+    exists (Maps.PTree.set _i (Vint (Int.repr (Z.of_nat 0))) le).
+    split.
+    - apply Maps.PTree.gss.
+    - repeat econstructor.
+    + rewrite PTree.gso. apply H0. eapply Pos.succ_discr. 
+    + apply PTree.gss.
+    + repeat econstructor.
+    + simpl. rewrite <- ptr_ofs_eq. apply H3.
+    + cbn. rewrite -> H4. reflexivity.
+    + cbn. unfold Val.of_bool. simpl in H8. rewrite H4 in H3.  rewrite Z.add_0_r in H8.  rewrite H8 in H3. inversion H3. reflexivity.
+    + Hypothesis fls : negb (Int.eq Int.zero Int.zero) = false.
+      rewrite fls. econstructor.
+    + apply PTree.gss.
+      (* Ind step *)
+     -   intros.
+        inversion H. unfold chunk in *. destruct H4.
+        eexists.
+        exists (Maps.PTree.set _i (Vint (Int.repr (Z.of_nat (S n)))) le).
+    split.
+      + apply Maps.PTree.gss.
+    + repeat econstructor.
+     rewrite PTree.gso. apply H0. eapply Pos.succ_discr. 
+     apply PTree.gss.
+     repeat econstructor.
+     simpl. rewrite <- ptr_ofs_eq. apply H3.
+     cbn. rewrite -> H4. reflexivity.
+     cbn. unfold Val.of_bool. simpl in H8. rewrite H4 in H3. destruct (negb (Int.eq x (Int.repr 0))). simpl.  Hypothesis tr : negb (Int.eq Int.one Int.zero) = true. rewrite tr. constructor. simpl. rewrite fls. (* false goal: prove the correctness of the loop *) 
+Admitted.
+
+(* Tactic for inversion  *)
+
+ Ltac invertSem :=
+        match goal with
+          | [H : context[exec_stmt] |- _] =>
+            inversion H ; clear H 
+          | [H : context[eval_expr] |- _] =>
+            inversion H ; clear H
+          | [H : context[eval_lvalue] |- _] =>
+            inversion H ; clear H 
+          | [H : context[bool_val] |- _] =>
+            inversion H ; clear H
+          | [H : context[deref_loc] |- _] =>
+            inversion H ; clear H  
+          | [H : context[sem_binary_operation] |- _] =>
+            inversion H ; clear H  
+          | [H : context[access_mode] |- _] =>
+            inversion H ; clear H  
+          | _ => idtac
+        end.    
+ 
+
+ Ltac solve_by_inverts n :=
+   match n with
+   | O => idtac
+   | S (?n') => invertSem ; subst ; solve_by_inverts n'
+   end.
+
+ (* behaves differently than the above: 
+
+  Ltac invert_clear :=
+        match goal with
+          | [H : context[exec_stmt] |- _] =>
+            inversion_clear H 
+          | [H : context[eval_expr] |- _] =>
+            inversion_clear H 
+          | [H : context[eval_lvalue] |- _] =>
+            inversion_clear H 
+          | [H : context[bool_val] |- _] =>
+            inversion_clear H  
+          | [H : context[deref_loc] |- _] =>
+            inversion_clear H  
+          | [H : context[sem_binary_operation] |- _] =>
+           inversion_clear H  
+          | [H : context[access_mode] |- _] =>
+            inversion_clear H  
+          | _ => idtac
+        end.    
+
+
+ Ltac solve_by_inverts n :=
+   match n with
+   | O => subst
+   | S (?n') =>  invert_clear; solve_by_inverts n'
+   end.
+
+  *)
+ 
+ Definition strlen_C_rel_corr_l : forall n m b ofs e le,
+     (n < INTSIZE)%nat ->
+     le!_s = Some (Vptr b (Ptrofs.repr ofs)) ->
+     (exists le', le'!_i = Some (Vint (Int.repr (Z_of_nat n))) /\ 
+                bigStepExec ge e le m f_strlen.(fn_body) t le' m (Out_return (Some (Vint (Int.repr (Z_of_nat n)),tuint))))
+           -> strlen_C_spec m b ofs (Some (n,m)).
+Proof.
+  intros.
+  repeat destruct H1.
+  inversion H2.
+  solve_by_inverts 5%nat. solve_by_inverts 15%nat. (* TODO: fix the tactic *)  Admitted.
+
+
+Definition strlen_C_exec_corr_l :
+  forall (m : Mem.mem) (b : block) (ofs : Z) (e : env) (le : temp_env) (z : Z),
+    le!_s = Some (Vptr b (Ptrofs.repr ofs)) -> 
+    (exists le', le'!_i = Some (Vint (Int.repr z)) /\ 
+                bigStepExec ge e le m f_strlen.(fn_body) t le' m (Out_return (Some (Vint (Int.repr z),tuint))))
+           -> strlen_C m b ofs = Some (z,m).
+Proof.
+  intros.
+  repeat destruct H0.
+  inversion H1.
+  solve_by_inverts 5%nat. solve_by_inverts 15%nat. 
+  unfold strlen_C.  unfold strlen_fun_C. unfold Mem.loadv in H9.
+  Admitted.
+              
+(* Examples of running a program: to see what assumptions need in the proof, experiments *)
+
+Parameter hi : Z.
+Definition init_mem := fst (Mem.alloc Mem.empty 0 hi).
+Definition b' := snd (Mem.alloc Mem.empty 0 hi).
+Parameter ofs' : Z.
+Hypothesis ofs_le_hi : ofs' < hi.
+
+(* Example 1 : output on empty string is correct *)
+
+Definition init_mem1 := 
+  Mem.store Mint8signed init_mem b' ofs' (Vint (Int.repr 0)).
+
+
+Lemma example_comp : forall m le e, init_mem1 = Some m ->
+                             le!_s = Some (Vptr b' (Ptrofs.repr ofs')) ->
+                             exists le', bigStepExec ge e le m f_strlen.(fn_body) t le' m (Out_return (Some (Vint (Int.repr 0),tuint))).
+Proof.
+  intros.
+  exists (Maps.PTree.set _i (Vint (Int.repr 0)) le).
+  repeat econstructor.
+    + rewrite PTree.gso. apply H0. eapply Pos.succ_discr. 
+    + apply Maps.PTree.gss.
+    + econstructor.
+    + unfold init_mem1 in H. simpl. rewrite (Mem.load_store_same  Mint8signed init_mem b' _ (Vint (Int.repr 0))). constructor. rewrite <- ptr_ofs_eq. assumption.
+    + econstructor.
+    + econstructor.
+    + econstructor.
+    + apply Maps.PTree.gss.
+Qed. 
+
+(* Running on a non-empty string: TODO prove the loop  *)
+
+Definition init_mem0 := fst (Mem.alloc Mem.empty 0 hi).
+Definition init_mem2 := Mem.store Mint8signed init_mem0 b' ofs' (Vint (Int.repr 1)).
+Definition init_mem3 := match init_mem2 with
+                        | None => None
+                        | Some m => Mem.store Mint8signed m b' (ofs'+1) (Vint (Int.repr 0))
+                        end.
+
+Lemma example_comp2 : forall m le e,
+                          init_mem2 = Some m ->
+                          init_mem3 = Some m -> 
+                          le!_s = Some (Vptr b' (Ptrofs.repr ofs')) ->
+                          exists le', bigStepExec ge e le m f_strlen.(fn_body) t le' m (Out_return (Some (Vint (Int.repr 1),tuint))).
+Proof.
+  intros.
+  exists (Maps.PTree.set _i (Vint (Int.repr 1)) le).
+  repeat econstructor.
+    + rewrite PTree.gso. apply H1. eapply Pos.succ_discr. 
+    + apply Maps.PTree.gss.
+    + econstructor.
+    + unfold init_mem3 in H0. rewrite H in H0. simpl. rewrite <- ptr_ofs_eq.
+      unfold init_mem2 in H. rewrite <- H in H0. rewrite -> (Mem.load_store_same Mint8signed init_mem0 b' ofs' (Vint (Int.repr 1))). econstructor. assumption.
+    + econstructor.      
+    + econstructor.
+    + Print exec_stmt. admit. 
+Admitted.
+
+     
+(** [deref_loc ty m b ofs v] computes the value of a datum
+  of type [ty] residing in memory [m] at block [b], offset [ofs].
+  If the type [ty] indicates an access by value, the corresponding
+  memory load is performed.  If the type [ty] indicates an access by
+  reference or by copy, the pointer [Vptr b ofs] is returned. *)
+
+
+
+(* 
+
+                                                
+   
+      
+  
+Lemma strlen_loop_continue_correct : Archi.ptr64 = false -> forall z ge e m b ofs outp le,
+      1 <= Z.of_nat outp + 1 < Ptrofs.modulus ->
+      0 < z ->
+      ofs + Z.of_nat outp < Ptrofs.modulus ->
+      0 < ofs < Ptrofs.modulus ->
+      1 <= Z.of_nat outp < Ptrofs.modulus ->
+      le!_input = Some (Vptr b (Ptrofs.repr ofs)) ->
+      le!_output = Some (Vint_of_nat outp) ->
+      Mem.load Mint8signed m b (ofs + (Z_of_nat outp)) = Some (Vint (Int.repr z)) ->
+      exists t le', exec_stmt ge e le m f_strlen_loop t le' m Out_normal /\
+               (le'!_output) = Some (Vint_of_nat (outp + 1)).
+
+Proof.
+  intro Arch.
+  intros z ge e m b ofs outp le.
+  intro P.
+  intro Z.
+  intro S.
+  intros.
+  repeat eexists.
+  Print exec_stmt.
+  - eapply exec_Sloop_loop.
+
+    eapply exec_Sifthenelse. econstructor. econstructor. econstructor.
+    econstructor.
+    econstructor.
+    apply H1.
+    econstructor.
+    apply H2. econstructor. econstructor. econstructor. simpl.
+    assert ( (Ptrofs.unsigned
+       (Ptrofs.add (Ptrofs.repr ofs)
+                   (Ptrofs.mul (Ptrofs.repr 1) (Ptrofs.of_intu (Int.repr (Z.of_nat outp)))))) = (ofs + (Z_of_nat outp)) ) as E1. 
+    { pose (Ptrofs.modulus_eq32 Arch).
+      rewrite Ptrofs.mul_commut. rewrite Ptrofs.mul_one. unfold Ptrofs.add. repeat rewrite Ptrofs.unsigned_repr_eq.  unfold Ptrofs.of_intu. unfold Ptrofs.of_int. repeat rewrite Int.unsigned_repr_eq. repeat rewrite Ptrofs.unsigned_repr_eq. repeat rewrite Zmod_small ; nia. }
+    rewrite E1. apply H3.
+    econstructor.
+    econstructor. simpl.
+    cut ((negb (Int.eq (Int.repr z) (Int.repr 0))) = true). intro aux. rewrite aux. simpl. econstructor. {  admit. }
+    econstructor.
+    econstructor.
+    econstructor.
+    econstructor. 
+   
+    econstructor.
+    apply H2.
+     econstructor.
+     econstructor.
+     eapply exec_Sloop_stop1. repeat econstructor. rewrite PTree.gso. apply H1. cbv. congruence. 
+     apply PTree.gss. econstructor. simpl.
+
+      assert ( 
+    (Ptrofs.unsigned
+       (Ptrofs.add (Ptrofs.repr ofs)
+          (Ptrofs.mul (Ptrofs.repr 1)
+             (Ptrofs.of_intu (Int.add (Int.repr (Z.of_nat outp)) (Int.repr 1)))))) = (ofs + (Z_of_nat outp + 1)) ) as E1. 
+    { pose (Ptrofs.modulus_eq32 Arch).
+      rewrite Ptrofs.mul_commut. rewrite Ptrofs.mul_one. unfold Ptrofs.add. repeat rewrite Ptrofs.unsigned_repr_eq.  unfold Ptrofs.of_intu. unfold Ptrofs.of_int. repeat rewrite Int.unsigned_repr_eq. repeat rewrite Ptrofs.unsigned_repr_eq. repeat rewrite Zmod_small; unfold Int.add; repeat rewrite Int.unsigned_repr_eq ;  repeat rewrite Zmod_small;  admit. } 
+    rewrite E1. (* Mem.load Mint8signed m b (ofs + (Z.of_nat outp + 1)) = Some ?v10 *)
+
+                                                                       
+
+Admitted.
+
+ *)
