c/poc/strlen_spec.v
@@ -262,6 +262,66 @@ Proof.
   - eapply gss.
 Qed.
 
+
+Lemma strlen_correct_loop_empty_string :
+  (* with this assumption Ptrofs.modulus = Int.modulus, ptherwise Ptrofs.modulus > Int.modulus *)
+  Archi.ptr64 = false ->
+  forall ge e m b ofs le len,                       
+    (* Preconditions on the length of the string and valid offset *)
+    0 < ofs < Ptrofs.modulus ->
+    Z_of_nat len < Int.modulus ->
+    ofs + Z_of_nat len < Ptrofs.modulus ->                      
+    (* Initialize local variables *)
+    le!_input = Some (Vptr b (Ptrofs.repr ofs)) ->
+    le!_output = Some (VintZ 0) ->                     
+    (* Precondition: reading empty C string from memory *)
+    strlen_mem m b ofs O ->
+    (* C light expression f_strlen returns O and assigns O to output variable *)
+    exists t le', exec_stmt ge e le m f_strlen_loop t le' m Out_normal /\ (le'!_output) = Some (VintN O).
+Proof.
+  intros.
+  inversion_clear H5.
+  repeat eexists.
+  - eapply exec_Sloop_stop1. (* break from the loop *)
+    repeat econstructor. 1,2: gso_assumption.
+    repeat econstructor. simpl.
+    replace (Ptrofs.unsigned
+               (Ptrofs.add (Ptrofs.repr ofs) (Ptrofs.mul (Ptrofs.repr 1) (Ptrofs.of_intu (Int.repr 0))))) with ofs.  apply H6. { pose (Ptrofs.modulus_eq32 H). ptrofs_compute_add_mul. all: nia. }
+   repeat econstructor. simpl. repeat econstructor. econstructor. econstructor.    
+  - assumption.
+Qed.
+
+
+Lemma strlen_correct_loop_empty_string1 :
+  (* with this assumption Ptrofs.modulus = Int.modulus, ptherwise Ptrofs.modulus > Int.modulus *)
+  Archi.ptr64 = false ->
+  forall ge e m b ofs le len,                       
+    (* Preconditions on the length of the string and valid offset *)
+    0 < ofs < Ptrofs.modulus ->
+    Z_of_nat len < Int.modulus ->
+    ofs + Z_of_nat len < Ptrofs.modulus ->                      
+    (* Initialize local variables *)
+    le!_input = Some (Vptr b (Ptrofs.repr ofs)) ->
+    le!_output = Some (VintZ 0) ->                     
+    (* Precondition: reading empty C string from memory *)
+    strlen_mem m b ofs O ->
+    (* C light expression f_strlen returns O and assigns O to output variable *)
+    exists t, exec_stmt ge e le m f_strlen_loop t le m Out_normal.
+Proof.
+  intros.
+ 
+
+  inversion_clear H5.
+   eexists.
+  - eapply exec_Sloop_stop1. (* break from the loop *)
+    repeat econstructor. 1,2: gso_assumption.
+    repeat econstructor. simpl.
+    replace (Ptrofs.unsigned
+               (Ptrofs.add (Ptrofs.repr ofs) (Ptrofs.mul (Ptrofs.repr 1) (Ptrofs.of_intu (Int.repr 0))))) with ofs. apply H6. { pose (Ptrofs.modulus_eq32 H). ptrofs_compute_add_mul. all: nia. }
+   repeat econstructor. simpl. repeat econstructor. econstructor. econstructor.    
+
+Qed.
+
 (* Conditions about the f_strlen loop *)
 (* If 0 is read from memory at [b,ofs + len] the output is set to len *)
 Lemma strlen_loop_break_correct : Archi.ptr64 = false -> forall ge e m b ofs outp le,
@@ -374,9 +434,6 @@ Proof.
     apply (IHlen m b (ofs + 1) H0).
 Qed.
 
-Lemma strlen_trans2 : forall len m b ofs, strlen_mem m b ofs (S len) -> strlen_mem m b (ofs + 1) len.
-Proof. intros. inversion H. assumption. Qed.
-
 Lemma strlen_trans3 : forall len m b ofs, strlen_mem m b ofs len -> forall i, (i < len)%nat -> strlen_mem m b (ofs + Z.of_nat i) (len - i)%nat.
 Proof.
   induction len.
@@ -405,39 +462,82 @@ Proof.
 Qed.
     
 
-Lemma strlen_loop_continue_correct : Archi.ptr64 = false -> forall len ge e m b ofs le,
-      
-      1 <= Z.of_nat (S len) < Ptrofs.modulus ->
-      ofs + Z.of_nat (S len) < Ptrofs.modulus ->
-      0 < ofs < Ptrofs.modulus ->
-      0 <= Z.of_nat (S len) < Ptrofs.modulus ->
+(* Lemma used in the induction step below *)
 
-      strlen_mem m b ofs len -> (* assume we have a string of length len at [b,ofs] in m *)
-      
-      forall i, (i < len)%nat ->  (* then the loop continues until len and outputs i++ *)
-           
-      le!_input = Some (Vptr b (Ptrofs.repr (ofs + Z.of_nat i))) -> (* ofs + i? *)
-      le!_output = Some (VintN i) ->
-      
-      exists t le', exec_stmt ge e le m f_strlen_loop t le' m Out_normal /\ le'!_output = Some (VintN (S i)).
+(* if executing f_strlen_loop with output = 0 and input = [b,ofs + 1] outputs len
+    then executing f_strlen_loop with output = 0 and input = [b,ofs] outputs (S outp) *)
+Lemma exec_trans : forall ge e le m t b ofs len,   
+    le!_output = Some (VintZ 0) ->
+    
+    exec_stmt ge e (PTree.set _input (Vptr b (Ptrofs.repr (ofs + 1))) le) m f_strlen_loop t  (PTree.set _output (VintN len)(PTree.set _input (Vptr b (Ptrofs.repr (ofs + 1))) le)) m Out_normal ->
+
+    le ! _input = Some (Vptr b (Ptrofs.repr ofs)) ->
+    (exists p : positive, Mem.load chunk m b ofs = Some (VintP p)) ->
+    exec_stmt ge e le m f_strlen_loop t (PTree.set _output (VintN (S len)) le) m Out_normal.
 Proof.
-  induction len.
-  - intros. omega.
-  - induction i.
-    + intros. inversion_clear H4.
-      pose (IHlen ge e m b (ofs + 1) le).
-      assert (1 <= Z.of_nat (S len) < Ptrofs.modulus) by nia. 
-      assert (ofs + 1 + Z.of_nat (S len) < Ptrofs.modulus) by nia.
-      assert (0 < ofs + 1 < Ptrofs.modulus) by nia.
-      assert (0 <= Z.of_nat (S len) < Ptrofs.modulus) by nia.
-      apply (e0 H4 H10 H11 H12).
-      assumption.
-      admit. (* (0 < len)%nat *) 
-      admit. (* le ! _input = Some (Vptr b (Ptrofs.repr (ofs + 1))) *)
-      assumption.
-    +   
-       
-Admitted.
+  (* (* loop *)
+      loop. repeat econstructor. repeat gso_assumption. gso_assumption. repeat econstructor. simpl. replace (Ptrofs.unsigned (Ptrofs.add (Ptrofs.repr ofs) (Ptrofs.mul (Ptrofs.repr 1) (Ptrofs.of_intu (Int.repr 0))))) with (ofs).
+   
+   apply H7.
+  { pose (Ptrofs.modulus_eq32 H). ptrofs_compute_add_mul. all: nia. } repeat econstructor. simpl. repeat econstructor. simpl.
+        replace (negb (Int.eq (Int.repr (Z.pos x0)) (Int.repr 0))) with true.      
+        econstructor. admit. repeat econstructor. econstructor. repeat econstructor.
+        gso_assumption. repeat econstructor.
+
+        fold f_strlen_loop. *) 
+  Admitted.
+
+Lemma strlen_loop_correct : (* with this assumption Ptrofs.modulus = Int.modulus, ptherwise Ptrofs.modulus > Int.modulus *)
+  Archi.ptr64 = false ->
+  forall len ge e m b ofs le,
+                       
+    (* Preconditions on the length of the string and valid offset *)
+    0 < ofs < Ptrofs.modulus ->
+    Z_of_nat len < Int.modulus ->
+    ofs + Z_of_nat len < Ptrofs.modulus ->
+                       
+                       (* Initialize local variables *)
+    le!_input = Some (Vptr b (Ptrofs.repr ofs)) ->
+    le!_output = Some (VintZ 0) ->
+                       
+       (* Precondition: reading C string of length len from memory *)
+    strlen_mem m b ofs len ->
+               
+      exists t, exec_stmt ge e le m f_strlen_loop t (PTree.set _output (VintN len) le) m Out_normal.
+Proof.
+   induction len ; intros.
+   (* Base case *)
+   -
+     assert ((PTree.set _output (VintN 0) le) = le). (* true *)
+     admit.
+     rewrite H6.  
+     eapply (strlen_correct_loop_empty_string1 _ _ _ _ _ ofs _ O). 1-3: nia. 1,2: gso_assumption. assumption.
+   
+  (* Inductive Step *)  
+  -  pose (strlen_trans4 (S len) m b ofs H5).
+
+  assert (exists t, exec_stmt ge e (PTree.set _input (Vptr b (Ptrofs.repr (ofs + 1))) le) m f_strlen_loop t
+       (PTree.set _output (VintN len) (PTree.set _input (Vptr b (Ptrofs.repr (ofs + 1))) le)) m
+       Out_normal).
+  
+  (* assert (exists (t : trace) (le' : temp_env),
+            exec_stmt ge e (PTree.set _input (Vptr b (Ptrofs.repr (ofs + 1))) le) m f_strlen_loop t le' m Out_normal /\
+            le' ! _output = Some (VintN len)). *)
+  refine (IHlen ge e m b (ofs + 1) (PTree.set _input (Vptr b (Ptrofs.repr (ofs + 1))) le)  _ _ _ _ _ _). 1-3: nia.  apply gss. gso_assumption. assumption. gso_assumption.
+  inversion_clear H5.
+  assumption.
+  destruct H6. (* destruct H6. destruct H6. *)
+
+  (* using lemmas *)
+  assert (0 < S len)%nat as L by omega.
+  destruct (e0 O L).  replace (ofs + Z.of_nat 0) with ofs in H7 by nia.  
+  repeat eexists.
+     -- pose (exec_trans ge e le m x b ofs len H4).
+        assert (exists p : positive,
+        Mem.load chunk m b ofs = Some (VintP p)) as J. exists x0. assumption.
+        pose (e1 H6 H3 J).
+        apply e2.  
+Admitted.        
 
 Lemma strlen_correct : (* with this assumption Ptrofs.modulus = Int.modulus, ptherwise Ptrofs.modulus > Int.modulus *)
   Archi.ptr64 = false ->
@@ -454,326 +554,23 @@ Lemma strlen_correct : (* with this assumption Ptrofs.modulus = Int.modulus, pth
                        
        (* Precondition: reading C string of length len from memory *)
     strlen_mem m b ofs len ->
-    
-           
-      exists t le', exec_stmt ge e le m f_strlen.(fn_body) t le' m (Out_return (Some ((VintN len),tuint))) /\ (le'!_output) = Some (VintN len).
+               
+      exists t le', exec_stmt ge e le m f_strlen.(fn_body) t le' m (Out_return (Some ((VintN len),tuint))).
 Proof.
   intros.
-  pose (S := strlen_trans len m b ofs H5).
-  inversion_clear S. 
-  
-  induction len.
-  
-  (* Base case *)
-  - intros. inversion_clear H5. eapply strlen_correct_empty_string. apply H. apply H0. apply H1. assumption. repeat gso_assumption. gso_assumption. apply H6.
-    
-  (* Inductive Step *)  
-  - intros.
-     pose (S := IHlen ge e m b (ofs + 1) le).
-    assert (0 < ofs + 1 < Ptrofs.modulus). nia.
-    assert (ofs + 1 + Z.of_nat len < Ptrofs.modulus). nia.
-    assert (Z.of_nat  len < Int.modulus). nia.
-    inversion_clear H5.
-    cut (le ! _input = Some (Vptr b (Ptrofs.repr (ofs + 1)))). intro.
-    pose ( S H6 H8 H7 H5 H4 H9  ).
-
-    pose (S := ). *)
-    inversion_clear H5. 
-   repeat eexists.
-      -- seq1.
+  destruct ( strlen_loop_correct H len ge e _ _ _ _ H0 H1 H2 H3 H4 H5).
+  eexists.
+  exists (PTree.set _output (VintN len) le). 
+   -- seq1.
          + seq1.
            * sset. repeat econstructor.
-           * fold f_strlen_loop. 
+           * fold f_strlen_loop.            
              
-Admitted. 
-                        
-(* Old stuff: One direction of correctness, using functional spec, below relational with proof attempt *)
+              assert ((PTree.set _output (Vint (Int.repr 0)) le) = le). 
+              { admit. (* true *) }
+              rewrite -> H7.
+              apply H6.
+         + repeat econstructor. apply gss.
+   Admitted.
+               
 
- Definition strlen_C_fun_corr_r :
-  forall (ge :genv) (m : Mem.mem) (b : block) (ofs : Z) (e : env) (le : temp_env) (z : Z),
-    strlen_C_fun_spec m b ofs = Some (z,m) ->
-    le!_s = Some (Vptr b (Ptrofs.repr ofs)) -> (* input parameter _s assigned value of address (b,ofs) in le *)
-    exists t le', exec_stmt ge e le m f_strlen.(fn_body) t le' m (Out_return (Some (Vint (Int.repr z),tuint))) /\ le'!_i = Some (Vint (Int.repr z)).
-               (* in environments ge, e (local env), le and memory m with output trace t, output _i assigned value z *)
-Proof.
-  intros.
-  repeat eexists.
-  (* econstructor can choose a wrong case in exec_stmt *)
-  eapply exec_Sseq_1. eapply exec_Sseq_1. econstructor. econstructor.
-  (* loop *)
-  (* - apply Maps.PTree.gss.
-    - repeat econstructor.
-    + rewrite PTree.gso. apply H0. eapply Pos.succ_discr. 
-    + apply PTree.gss.
-    + repeat econstructor. *)
-Admitted.
-
- (* Find proofs on arithmetic on ptrofs type to rewrite this *)
-      Hypothesis ptr_ofs_eq : forall ofs, ofs = (Ptrofs.unsigned
-       (Ptrofs.add (Ptrofs.repr ofs)
-                   (Ptrofs.mul (Ptrofs.repr 1) (Ptrofs.of_intu (Int.repr 0))))). 
-
-      
-Definition strlen_C_rel_corr_r : forall n m b ofs e le ge,
-    strlen_C_rel_spec m b ofs (Some (n,m)) ->
-    le!_s = Some (Vptr b (Ptrofs.repr ofs)) -> 
-    exists t le', le'!_i = Some (Vint_of_nat n) /\ 
-           exec_stmt ge e le m f_strlen.(fn_body) t le' m (Out_return (Some ((Vint_of_nat n),tuint))).
-Proof.
-  induction n.
-  (* Base case. *)
-    intros.
-    inversion H. unfold chunk in *. destruct H4.
-    eexists.
-    exists (Maps.PTree.set _i (Vint (Int.repr (Z.of_nat 0))) le).
-    split.
-    - apply Maps.PTree.gss.
-    - repeat econstructor.
-    + rewrite PTree.gso. apply H0. eapply Pos.succ_discr. 
-    + apply PTree.gss.
-    + repeat econstructor.
-    + simpl. rewrite <- ptr_ofs_eq. apply H3.
-    + cbn. rewrite -> H4. reflexivity.
-    + cbn. unfold Val.of_bool. simpl in H8. rewrite H4 in H3.  rewrite Z.add_0_r in H8.  rewrite H8 in H3. inversion H3. reflexivity.
-    + Hypothesis fls : negb (Int.eq Int.zero Int.zero) = false.
-      rewrite fls. econstructor.
-    + apply PTree.gss.
-      (* Ind step *)
-     -   intros.
-        inversion H. unfold chunk in *. destruct H4.
-        eexists.
-        exists (Maps.PTree.set _i (Vint (Int.repr (Z.of_nat (S n)))) le).
-    split.
-      + apply Maps.PTree.gss.
-    + repeat econstructor.
-     rewrite PTree.gso. apply H0. eapply Pos.succ_discr. 
-     apply PTree.gss.
-     repeat econstructor.
-     simpl. rewrite <- ptr_ofs_eq. apply H3.
-     cbn. rewrite -> H4. reflexivity.
-     cbn. unfold Val.of_bool. simpl in H8. rewrite H4 in H3. destruct (negb (Int.eq x (Int.repr 0))). simpl.  Hypothesis tr : negb (Int.eq Int.one Int.zero) = true. rewrite tr. constructor. simpl. rewrite fls. (* false goal: prove the correctness of the loop *) 
-Admitted.
-
-(* Tactic for inversion  *)
-
- Ltac invertSem :=
-        match goal with
-          | [H : context[exec_stmt] |- _] =>
-            inversion H ; clear H 
-          | [H : context[eval_expr] |- _] =>
-            inversion H ; clear H
-          | [H : context[eval_lvalue] |- _] =>
-            inversion H ; clear H 
-          | [H : context[bool_val] |- _] =>
-            inversion H ; clear H
-          | [H : context[deref_loc] |- _] =>
-            inversion H ; clear H  
-          | [H : context[sem_binary_operation] |- _] =>
-            inversion H ; clear H  
-          | [H : context[access_mode] |- _] =>
-            inversion H ; clear H  
-          | _ => idtac
-        end.    
- 
-
- Ltac solve_by_inverts n :=
-   match n with
-   | O => idtac
-   | S (?n') => invertSem ; subst ; solve_by_inverts n'
-   end.
-
- (* behaves differently than the above: 
-
-  Ltac invert_clear :=
-        match goal with
-          | [H : context[exec_stmt] |- _] =>
-            inversion_clear H 
-          | [H : context[eval_expr] |- _] =>
-            inversion_clear H 
-          | [H : context[eval_lvalue] |- _] =>
-            inversion_clear H 
-          | [H : context[bool_val] |- _] =>
-            inversion_clear H  
-          | [H : context[deref_loc] |- _] =>
-            inversion_clear H  
-          | [H : context[sem_binary_operation] |- _] =>
-           inversion_clear H  
-          | [H : context[access_mode] |- _] =>
-            inversion_clear H  
-          | _ => idtac
-        end.    
-
-
- Ltac solve_by_inverts n :=
-   match n with
-   | O => subst
-   | S (?n') =>  invert_clear; solve_by_inverts n'
-   end.
-
-  *)
- 
- Definition strlen_C_rel_corr_l : forall n m b ofs e le,
-     (n < INTSIZE)%nat ->
-     le!_s = Some (Vptr b (Ptrofs.repr ofs)) ->
-     (exists le', le'!_i = Some (Vint (Int.repr (Z_of_nat n))) /\ 
-                bigStepExec ge e le m f_strlen.(fn_body) t le' m (Out_return (Some (Vint (Int.repr (Z_of_nat n)),tuint))))
-           -> strlen_C_spec m b ofs (Some (n,m)).
-Proof.
-  intros.
-  repeat destruct H1.
-  inversion H2.
-  solve_by_inverts 5%nat. solve_by_inverts 15%nat. (* TODO: fix the tactic *)  Admitted.
-
-
-Definition strlen_C_exec_corr_l :
-  forall (m : Mem.mem) (b : block) (ofs : Z) (e : env) (le : temp_env) (z : Z),
-    le!_s = Some (Vptr b (Ptrofs.repr ofs)) -> 
-    (exists le', le'!_i = Some (Vint (Int.repr z)) /\ 
-                bigStepExec ge e le m f_strlen.(fn_body) t le' m (Out_return (Some (Vint (Int.repr z),tuint))))
-           -> strlen_C m b ofs = Some (z,m).
-Proof.
-  intros.
-  repeat destruct H0.
-  inversion H1.
-  solve_by_inverts 5%nat. solve_by_inverts 15%nat. 
-  unfold strlen_C.  unfold strlen_fun_C. unfold Mem.loadv in H9.
-  Admitted.
-              
-(* Examples of running a program: to see what assumptions need in the proof, experiments *)
-
-Parameter hi : Z.
-Definition init_mem := fst (Mem.alloc Mem.empty 0 hi).
-Definition b' := snd (Mem.alloc Mem.empty 0 hi).
-Parameter ofs' : Z.
-Hypothesis ofs_le_hi : ofs' < hi.
-
-(* Example 1 : output on empty string is correct *)
-
-Definition init_mem1 := 
-  Mem.store Mint8signed init_mem b' ofs' (Vint (Int.repr 0)).
-
-
-Lemma example_comp : forall m le e, init_mem1 = Some m ->
-                             le!_s = Some (Vptr b' (Ptrofs.repr ofs')) ->
-                             exists le', bigStepExec ge e le m f_strlen.(fn_body) t le' m (Out_return (Some (Vint (Int.repr 0),tuint))).
-Proof.
-  intros.
-  exists (Maps.PTree.set _i (Vint (Int.repr 0)) le).
-  repeat econstructor.
-    + rewrite PTree.gso. apply H0. eapply Pos.succ_discr. 
-    + apply Maps.PTree.gss.
-    + econstructor.
-    + unfold init_mem1 in H. simpl. rewrite (Mem.load_store_same  Mint8signed init_mem b' _ (Vint (Int.repr 0))). constructor. rewrite <- ptr_ofs_eq. assumption.
-    + econstructor.
-    + econstructor.
-    + econstructor.
-    + apply Maps.PTree.gss.
-Qed. 
-
-(* Running on a non-empty string: TODO prove the loop  *)
-
-Definition init_mem0 := fst (Mem.alloc Mem.empty 0 hi).
-Definition init_mem2 := Mem.store Mint8signed init_mem0 b' ofs' (Vint (Int.repr 1)).
-Definition init_mem3 := match init_mem2 with
-                        | None => None
-                        | Some m => Mem.store Mint8signed m b' (ofs'+1) (Vint (Int.repr 0))
-                        end.
-
-Lemma example_comp2 : forall m le e,
-                          init_mem2 = Some m ->
-                          init_mem3 = Some m -> 
-                          le!_s = Some (Vptr b' (Ptrofs.repr ofs')) ->
-                          exists le', bigStepExec ge e le m f_strlen.(fn_body) t le' m (Out_return (Some (Vint (Int.repr 1),tuint))).
-Proof.
-  intros.
-  exists (Maps.PTree.set _i (Vint (Int.repr 1)) le).
-  repeat econstructor.
-    + rewrite PTree.gso. apply H1. eapply Pos.succ_discr. 
-    + apply Maps.PTree.gss.
-    + econstructor.
-    + unfold init_mem3 in H0. rewrite H in H0. simpl. rewrite <- ptr_ofs_eq.
-      unfold init_mem2 in H. rewrite <- H in H0. rewrite -> (Mem.load_store_same Mint8signed init_mem0 b' ofs' (Vint (Int.repr 1))). econstructor. assumption.
-    + econstructor.      
-    + econstructor.
-    + Print exec_stmt. admit. 
-Admitted.
-
-     
-(** [deref_loc ty m b ofs v] computes the value of a datum
-  of type [ty] residing in memory [m] at block [b], offset [ofs].
-  If the type [ty] indicates an access by value, the corresponding
-  memory load is performed.  If the type [ty] indicates an access by
-  reference or by copy, the pointer [Vptr b ofs] is returned. *)
-
-
-
-(* 
-
-                                                
-   
-      
-  
-Lemma strlen_loop_continue_correct : Archi.ptr64 = false -> forall z ge e m b ofs outp le,
-      1 <= Z.of_nat outp + 1 < Ptrofs.modulus ->
-      0 < z ->
-      ofs + Z.of_nat outp < Ptrofs.modulus ->
-      0 < ofs < Ptrofs.modulus ->
-      1 <= Z.of_nat outp < Ptrofs.modulus ->
-      le!_input = Some (Vptr b (Ptrofs.repr ofs)) ->
-      le!_output = Some (Vint_of_nat outp) ->
-      Mem.load Mint8signed m b (ofs + (Z_of_nat outp)) = Some (Vint (Int.repr z)) ->
-      exists t le', exec_stmt ge e le m f_strlen_loop t le' m Out_normal /\
-               (le'!_output) = Some (Vint_of_nat (outp + 1)).
-
-Proof.
-  intro Arch.
-  intros z ge e m b ofs outp le.
-  intro P.
-  intro Z.
-  intro S.
-  intros.
-  repeat eexists.
-  Print exec_stmt.
-  - eapply exec_Sloop_loop.
-
-    eapply exec_Sifthenelse. econstructor. econstructor. econstructor.
-    econstructor.
-    econstructor.
-    apply H1.
-    econstructor.
-    apply H2. econstructor. econstructor. econstructor. simpl.
-    assert ( (Ptrofs.unsigned
-       (Ptrofs.add (Ptrofs.repr ofs)
-                   (Ptrofs.mul (Ptrofs.repr 1) (Ptrofs.of_intu (Int.repr (Z.of_nat outp)))))) = (ofs + (Z_of_nat outp)) ) as E1. 
-    { pose (Ptrofs.modulus_eq32 Arch).
-      rewrite Ptrofs.mul_commut. rewrite Ptrofs.mul_one. unfold Ptrofs.add. repeat rewrite Ptrofs.unsigned_repr_eq.  unfold Ptrofs.of_intu. unfold Ptrofs.of_int. repeat rewrite Int.unsigned_repr_eq. repeat rewrite Ptrofs.unsigned_repr_eq. repeat rewrite Zmod_small ; nia. }
-    rewrite E1. apply H3.
-    econstructor.
-    econstructor. simpl.
-    cut ((negb (Int.eq (Int.repr z) (Int.repr 0))) = true). intro aux. rewrite aux. simpl. econstructor. {  admit. }
-    econstructor.
-    econstructor.
-    econstructor.
-    econstructor. 
-   
-    econstructor.
-    apply H2.
-     econstructor.
-     econstructor.
-     eapply exec_Sloop_stop1. repeat econstructor. rewrite PTree.gso. apply H1. cbv. congruence. 
-     apply PTree.gss. econstructor. simpl.
-
-      assert ( 
-    (Ptrofs.unsigned
-       (Ptrofs.add (Ptrofs.repr ofs)
-          (Ptrofs.mul (Ptrofs.repr 1)
-             (Ptrofs.of_intu (Int.add (Int.repr (Z.of_nat outp)) (Int.repr 1)))))) = (ofs + (Z_of_nat outp + 1)) ) as E1. 
-    { pose (Ptrofs.modulus_eq32 Arch).
-      rewrite Ptrofs.mul_commut. rewrite Ptrofs.mul_one. unfold Ptrofs.add. repeat rewrite Ptrofs.unsigned_repr_eq.  unfold Ptrofs.of_intu. unfold Ptrofs.of_int. repeat rewrite Int.unsigned_repr_eq. repeat rewrite Ptrofs.unsigned_repr_eq. repeat rewrite Zmod_small; unfold Int.add; repeat rewrite Int.unsigned_repr_eq ;  repeat rewrite Zmod_small;  admit. } 
-    rewrite E1. (* Mem.load Mint8signed m b (ofs + (Z.of_nat outp + 1)) = Some ?v10 *)
-
-                                                                       
-
-Admitted.
-
- *)
